Makefile
@@ -5,6 +5,8 @@ MODULES := MyTactics \
 
 VS 	:= $(MODULES:%=%.v)
 
+COQDOCFLAGS="--gallina --interpolate --utf8"
+
 .PHONY: coq doc clean
 
 all: coq doc
@@ -13,8 +15,7 @@ coq: Makefile.coq
 	$(MAKE) -f Makefile.coq
 
 Makefile.coq: Makefile $(VS:%=%)
-	echo $(VS)
-	coq_makefile $(VS) -o Makefile.coq
+	coq_makefile $(VS) COQDOCFLAGS = $(COQDOCFLAGS) -o Makefile.coq
 
 clean: Makefile.coq
 	$(MAKE) -f Makefile.coq clean
